\let\negmedspace\undefined
\let\negthickspace\undefined
\documentclass[journal]{IEEEtran}
\usepackage[a5paper, margin=10mm, onecolumn]{geometry}
%\usepackage{lmodern} % Ensure lmodern is loaded for pdflatex
\usepackage{tfrupee} % Include tfrupee package

\setlength{\headheight}{1cm} % Set the height of the header box
\setlength{\headsep}{0mm}     % Set the distance between the header box and the top of the text

\usepackage{gvv-book}
\usepackage{gvv}
\usepackage{cite}
\usepackage{amsmath,amssymb,amsfonts,amsthm}
\usepackage{algorithmic}
\usepackage{graphicx}
\usepackage{textcomp}
\usepackage{xcolor}
\usepackage{txfonts}
\usepackage{listings}
\usepackage{enumitem}
\usepackage{mathtools}
\usepackage{gensymb}
\usepackage{comment}
\usepackage[breaklinks=true]{hyperref}
\usepackage{tkz-euclide} 
\usepackage{listings}
% \usepackage{gvv}                                        
\def\inputGnumericTable{}                                 
\usepackage[latin1]{inputenc}                                
\usepackage{color}                                            
\usepackage{array}                                            
\usepackage{longtable}                                       
\usepackage{calc}                                             
\usepackage{multirow}                                         
\usepackage{hhline}                                           
\usepackage{ifthen}                                           
\usepackage{lscape}
\begin{document}

\bibliographystyle{IEEEtran}
\vspace{3cm}

\title{9.3.11.4}
\author{EE24BTECH11058 - P.Shiny Diavajna}
% \maketitle
% \newpage
% \bigskip
{\let\newpage\relax\maketitle}

\renewcommand{\thefigure}{\theenumi}
\renewcommand{\thetable}{\theenumi}
\setlength{\intextsep}{10pt} % Space between text and floats


\numberwithin{equation}{enumi}
\numberwithin{figure}{enumi}
\renewcommand{\thetable}{\theenumi}

\textbf{Question:} Solve the differential equation $\frac{d^2y}{dx^2}-1=0$ with initial conditions $y\brak{0}=0$ and $y^{\prime}\brak{0}=0$\\

\textbf{Theoretical Solution:}\\
Laplace Transform:
\begin{align}
    \mathcal{L}\brak{f(t)} = \int_{0}^{\infty}e^{-st}f(t)dt
\end{align}
Properties of Laplace Transform:
\begin{align}
    \mathcal{L}\brak{y^{\prime\prime}} &= s^2 \mathcal{L}\brak{y} -s y\brak{0} - y^{\prime}\brak{0}\\
    \mathcal{L}\brak{1}&= \frac{1}{s}\\
    \mathcal{L}^{-1}\brak{\frac{2}{s^3}}&=x^{2} u\brak{x}
\end{align}
Apply the properties to the given equation 
\begin{align}
     y^{\prime\prime}\brak{x}-1=0\\
     \mathcal{L}\brak{y^{\prime\prime}}-\mathcal{L}\brak{1}=0\\
     s^2 \mathcal{L}\brak{y}- sy\brak{0} - y^{\prime}\brak{0}-\frac{1}{s}=0
\end{align}

Substituting the initial conditions in equation $(0.8)$
\begin{align}
    s^3\mathcal{L}\brak{y}-1=0\\
    \mathcal{L}\brak{y}= \frac{1}{s^3}\\
    y=\mathcal{L}^{-1}\brak{\frac{1}{s^3}}\\
    y= \frac{x^2}{2} u\brak{x}
\end{align}

Theoretical solution is 
\begin{align}
    y(x) = \frac{x^2}{2} u\brak{x}
\end{align}

\textbf{Bilinear Transform:}
\begin{align}
    s=\frac{2}{h}.\frac{1-z^{-1}}{1+z^{-1}}
\end{align}
Substitute $(0.13)$ in $(0.9)$

\begin{align}
    Y\brak{z}&=\brak{\frac{h}{2}}^3 \brak{\frac{1+z^{-1}}{1-z^{-1}}}^3\\
    Y\brak{z}&=\brak{\frac{h}{2}}^3 \brak{\frac{1+3z^{-1}+3z^{-2}+z^{-3}}{1-3z^{-1}+3z^{-2}-z^{-3}}}\\
    Y\brak{z}\brak{1-3z^{-1}+3z^{-2}-z^{-3}}&=\brak{\frac{h}{2}}^3 \brak{1+3z^{-1}+3z^{-2}+z^{-3}}
\end{align}
Multiply the above equation with $z^3$ and take the inverse $z$ transform to obtain difference equation
\begin{align}
    y\brak{n+3}-3y\brak{n+2}+3y\brak{n+1}-y\brak{n}&=\brak{\frac{h}{2}}^3\brak{\delta\brak{n+3}+3\delta\brak{n+2}+3\delta\brak{n+1}+\delta\brak{n}}   
\end{align}
\begin{align}
    y\brak{n+3}-3y\brak{n+2}+3y\brak{n+1}-y\brak{n}&=\brak{\frac{h}{2}}^3 \delta\brak{n}-h^2\delta\brak{n}
\end{align}

\textbf{Computational Solution:}\\:
Method of finite differences:\\
The second derivative can be approximated as:
\begin{align}
    \frac{d^2y}{dx^2}=\frac{y_{n+1}-2y_n+y_{n-1}}{h^2}
\end{align}
Substitute this into the differential equation:
\begin{align}
    \frac{y_{n+1}-2y_n+y_{n+1}}{h^2}-1=0\\
    y_{n+1}=2y_{n}-y_{n-1}+h^2
\end{align}

Given $y\brak{0}=0$ and $y^{\prime}\brak{0}=0$
\begin{align}
    y_{1}&=y_{0}+y^{\prime}\brak{0}.h\\
    y_1&=0
\end{align}

This curve is generated by applying the finite difference method to the given problem and taking the values of $x_0=0,y_0=0,y_1=0$ and $h=0.001$ and running the iterations for 1000 times 

\begin{figure}[h]
   \centering
   \includegraphics[width=\columnwidth]{figs/fig.png}
\end{figure}

\end{document}

 

 
 
